src/computational_monads/simulation_semantics/query_cache/get_or_else.lean
@@ -3,7 +3,7 @@ Copyright (c) 2023 Devon Tuma. All rights reserved.
 Released under Apache 2.0 license as described in the file LICENSE.
 Authors: Devon Tuma
 -/
-import computational_monads.simulation_semantics.constructions.logging.query_cache.order
+import computational_monads.simulation_semantics.query_cache.order
 import computational_monads.distribution_semantics.ite
 import computational_monads.distribution_semantics.prod
 
