src/computational_monads/simulation_semantics/query_cache/sdiff.lean
@@ -1,0 +1,72 @@
+/-
+Copyright (c) 2023 Devon Tuma. All rights reserved.
+Released under Apache 2.0 license as described in the file LICENSE.
+Authors: Devon Tuma
+-/
+import computational_monads.simulation_semantics.query_cache.order
+
+/-!
+# Removing Cached Values from a Cache
+
+This file defines a `has_sdiff` instance on `query_cache`, where `cache \ cache'` is the result of
+dropping any values in `cache` that are also cached in `cache'`.
+The removal is independent of the actual values stored in the cache.
+-/
+
+namespace query_cache
+
+variables {spec : oracle_spec}
+
+/-- We define a diff operation `cache \ cache'` on `query_cache` by removing any cached elements
+in `cache'` from `cache`, leaving everything else unchanged. -/
+instance : has_sdiff (query_cache spec) :=
+{ sdiff := λ cache cache', {
+    cache_fn := λ i t, if cache'.is_fresh i t then cache.lookup i t else none,
+    cached_inputs := cache.cached_inputs \ cache'.cached_inputs,
+    mem_cached_inputs := λ x, by simp [and_comm, is_fresh_iff_not_mem_cached_inputs] } }
+
+variables (cache cache' : query_cache spec) (i : spec.ι) (t : spec.domain i)
+
+section lookup
+
+@[simp] lemma lookup_sdiff : (cache \ cache').lookup i t =
+  if cache'.is_fresh i t then cache.lookup i t else none := rfl
+
+lemma lookup_sdiff_eq_some_iff (u) : (cache \ cache').lookup i t = some u ↔
+  cache'.is_fresh i t ∧ cache.lookup i t = some u :=
+by by_cases h : cache'.is_fresh i t; simp [h]
+
+lemma lookup_sdiff_eq_none_iff : (cache \ cache').lookup i t = none ↔
+  cache.is_fresh i t ∨ cache'.is_cached i t :=
+by rw [lookup_sdiff, ite_eq_right_iff, lookup_eq_none_iff_is_fresh,
+  imp_iff_not_or, not_is_fresh_iff_is_cached, or_comm]
+
+end lookup
+
+@[simp] lemma init_sdiff : ∅ \ cache = ∅ := query_cache.extₗ (λ i t, if_t_t _ _)
+
+@[simp] lemma sdiff_init : cache \ ∅ = cache := query_cache.extₗ (λ i t, by simp)
+
+@[simp] lemma sdiff_self : cache \ cache = ∅ := query_cache.extₗ (λ i t, by simp)
+
+@[simp] lemma sdiff_cache_query (u) : [i, t ↦ u; cache] \ cache =
+  if cache.is_fresh i t then [i, t ↦ u] else ∅ :=
+begin
+  refine query_cache.extₗ (λ i' t', _),
+  by_cases hit : cache.is_fresh i t;
+  { by_cases hi : i = i',
+    { induction hi,
+      by_cases ht : t = t',
+      { simp [← ht, hit] },
+      { simp [ht, hit] } },
+    { simp [hi, hit] } },
+end
+
+lemma sdiff_le_fst : cache \ cache' ≤ cache :=
+begin
+  refine λ i t u hu, _,
+  rw [lookup_sdiff_eq_some_iff] at hu,
+  exact hu.2,
+end
+
+end query_cache
